theories/Symbolic/PartialEvaluation.v
@@ -56,116 +56,120 @@ Module Type PartialEvaluationOn
   Local Notation LCtx := (NCtx 𝑺 Ty).
   Local Notation Valuation Σ := (@Env (Binding 𝑺 Ty) (fun xt : Binding 𝑺 Ty => Val (@type 𝑺 Ty xt)) Σ).
 
-  Equations(noeqns) peval_append {Σ σ} (t1 t2 : Term Σ (ty_list σ)) : Term Σ (ty_list σ) :=
-  | term_val _ v1                 | term_val _ v2 := term_val (ty_list σ) (app v1 v2);
-  (* TODO: recurse over the value instead *)
-  | term_val _ nil                | t2 := t2;
-  | term_val _ (cons v vs)        | t2 := term_binop binop_cons (term_val σ v) (term_binop binop_append (term_val (ty_list σ) vs) t2);
-  | term_binop binop_cons t11 t12 | t2 := term_binop binop_cons t11 (term_binop binop_append t12 t2);
-  | t1                            | t2 := term_binop binop_append t1 t2.
+  Section WithLCtx.
+    Context {Σ : LCtx}.
 
-  Equations(noeqns) peval_binop' {Σ σ1 σ2 σ} (op : BinOp σ1 σ2 σ) (t1 : Term Σ σ1) (t2 : Term Σ σ2) : Term Σ σ :=
-  | op | term_val _ v1 | term_val _ v2 := term_val σ (eval_binop op v1 v2);
-  | op | t1            | t2            := term_binop op t1 t2.
+    Equations(noeqns) peval_append {σ} (t1 t2 : Term Σ (ty_list σ)) : Term Σ (ty_list σ) :=
+    | term_val _ v1                 | term_val _ v2 := term_val (ty_list σ) (app v1 v2);
+    (* TODO: recurse over the value instead *)
+    | term_val _ nil                | t2 := t2;
+    | term_val _ (cons v vs)        | t2 := term_binop binop_cons (term_val σ v) (term_binop binop_append (term_val (ty_list σ) vs) t2);
+    | term_binop binop_cons t11 t12 | t2 := term_binop binop_cons t11 (term_binop binop_append t12 t2);
+    | t1                            | t2 := term_binop binop_append t1 t2.
 
-  Equations(noeqns) peval_binop {Σ σ1 σ2 σ} (op : BinOp σ1 σ2 σ) (t1 : Term Σ σ1) (t2 : Term Σ σ2) : Term Σ σ :=
-  | binop_append | t1 | t2 := peval_append t1 t2;
-  | op           | t1 | t2 := peval_binop' op t1 t2.
+    Equations(noeqns) peval_binop' {σ1 σ2 σ} (op : BinOp σ1 σ2 σ) (t1 : Term Σ σ1) (t2 : Term Σ σ2) : Term Σ σ :=
+    | op | term_val _ v1 | term_val _ v2 := term_val σ (eval_binop op v1 v2);
+    | op | t1            | t2            := term_binop op t1 t2.
 
-  Lemma peval_append_sound {Σ σ} (t1 t2 : Term Σ (ty_list σ)) :
-    forall (ι : Valuation Σ),
-      inst  (peval_append t1 t2) ι =
-        eval_binop binop_append (inst t1 ι) (inst t2 ι).
-  Proof.
-    intros ι.
-    dependent elimination t1; cbn; auto.
-    - dependent elimination t2; cbn; auto;
-      destruct v; cbn; auto.
-    - dependent elimination op; cbn; auto.
-  Qed.
+    Equations(noeqns) peval_binop {σ1 σ2 σ} (op : BinOp σ1 σ2 σ) (t1 : Term Σ σ1) (t2 : Term Σ σ2) : Term Σ σ :=
+    | binop_append | t1 | t2 := peval_append t1 t2;
+    | op           | t1 | t2 := peval_binop' op t1 t2.
 
-  Lemma peval_binop'_sound {Σ σ1 σ2 σ} (op : BinOp σ1 σ2 σ) (t1 : Term Σ σ1) (t2 : Term Σ σ2) :
-    forall (ι : Valuation Σ),
-      inst (peval_binop' op t1 t2) ι = eval_binop op (inst t1 ι) (inst t2 ι).
-  Proof. intros ι. destruct t1, t2; cbn; auto. Qed.
+    Lemma peval_append_sound {σ} (t1 t2 : Term Σ (ty_list σ)) :
+      forall (ι : Valuation Σ),
+        inst  (peval_append t1 t2) ι =
+          eval_binop binop_append (inst t1 ι) (inst t2 ι).
+    Proof.
+      intros ι.
+      dependent elimination t1; cbn; auto.
+      - dependent elimination t2; cbn; auto;
+        destruct v; cbn; auto.
+      - dependent elimination op; cbn; auto.
+    Qed.
 
-  Lemma peval_binop_sound {Σ σ1 σ2 σ} (op : BinOp σ1 σ2 σ) (t1 : Term Σ σ1) (t2 : Term Σ σ2) :
-    forall (ι : Valuation Σ),
-      inst (peval_binop op t1 t2) ι = eval_binop op (inst t1 ι) (inst t2 ι).
-  Proof.
-    intros ι.
-    destruct op; cbn [peval_binop];
-      auto using peval_binop'_sound, peval_append_sound.
-  Qed.
+    Lemma peval_binop'_sound {σ1 σ2 σ} (op : BinOp σ1 σ2 σ) (t1 : Term Σ σ1) (t2 : Term Σ σ2) :
+      forall (ι : Valuation Σ),
+        inst (peval_binop' op t1 t2) ι = eval_binop op (inst t1 ι) (inst t2 ι).
+    Proof. intros ι. destruct t1, t2; cbn; auto. Qed.
 
-  Equations(noeqns) peval_neg {Σ} (t : Term Σ ty_int) : Term Σ ty_int :=
-  | term_val _ v := term_val ty_int (Z.opp v);
-  | t            := term_neg t.
+    Lemma peval_binop_sound {σ1 σ2 σ} (op : BinOp σ1 σ2 σ) (t1 : Term Σ σ1) (t2 : Term Σ σ2) :
+      forall (ι : Valuation Σ),
+        inst (peval_binop op t1 t2) ι = eval_binop op (inst t1 ι) (inst t2 ι).
+    Proof.
+      intros ι.
+      destruct op; cbn [peval_binop];
+        auto using peval_binop'_sound, peval_append_sound.
+    Qed.
 
-  Equations(noeqns) peval_not {Σ} (t : Term Σ ty_bool) : Term Σ ty_bool :=
-  | term_val _ v := term_val ty_bool (negb v);
-  | t            := term_not t.
+    Equations(noeqns) peval_neg (t : Term Σ ty_int) : Term Σ ty_int :=
+    | term_val _ v := term_val ty_int (Z.opp v);
+    | t            := term_neg t.
 
-  Equations(noeqns) peval_inl {Σ σ1 σ2} (t : Term Σ σ1) : Term Σ (ty_sum σ1 σ2) :=
-  | term_val _ v := term_val (ty_sum _ _) (@inl (Val _) (Val _) v);
-  | t            := term_inl t.
+    Equations(noeqns) peval_not (t : Term Σ ty_bool) : Term Σ ty_bool :=
+    | term_val _ v := term_val ty_bool (negb v);
+    | t            := term_not t.
 
-  Equations(noeqns) peval_inr {Σ σ1 σ2} (t : Term Σ σ2) : Term Σ (ty_sum σ1 σ2) :=
-  | term_val _ v := term_val (ty_sum _ _) (@inr (Val _) (Val _) v);
-  | t            := term_inr t.
+    Equations(noeqns) peval_inl {σ1 σ2} (t : Term Σ σ1) : Term Σ (ty_sum σ1 σ2) :=
+    | term_val _ v := term_val (ty_sum _ _) (@inl (Val _) (Val _) v);
+    | t            := term_inl t.
 
-  Equations(noeqns) peval {Σ σ} (t : Term Σ σ) : Term Σ σ :=
-  | term_var ς                 := term_var ς;
-  | term_val _ v               := term_val _ v;
-  | term_binop op t1 t2        := peval_binop op (peval t1) (peval t2);
-  | term_neg t                 := peval_neg (peval t);
-  | term_not t                 := peval_not (peval t);
-  | term_inl t                 := peval_inl (peval t);
-  | term_inr t                 := peval_inr (peval t);
-  (* TODO: Finish the cases below. *)
-  | @term_projtup _ _ t n _ p  := @term_projtup _ _ (peval t) n _ p;
-  | @term_union _ U K t        := @term_union _ U K (peval t);
-  | @term_record _ R ts        := @term_record _ R ts.
+    Equations(noeqns) peval_inr {σ1 σ2} (t : Term Σ σ2) : Term Σ (ty_sum σ1 σ2) :=
+    | term_val _ v := term_val (ty_sum _ _) (@inr (Val _) (Val _) v);
+    | t            := term_inr t.
 
-  Lemma peval_neg_sound {Σ} (t : Term Σ ty_int) :
-    forall (ι : Valuation Σ),
-      inst (peval_neg t) ι = inst (term_neg t) ι.
-  Proof. dependent elimination t; cbn; auto. Qed.
+    Equations(noeqns) peval [σ] (t : Term Σ σ) : Term Σ σ :=
+    | term_var ς                 := term_var ς;
+    | term_val _ v               := term_val _ v;
+    | term_binop op t1 t2        := peval_binop op (peval t1) (peval t2);
+    | term_neg t                 := peval_neg (peval t);
+    | term_not t                 := peval_not (peval t);
+    | term_inl t                 := peval_inl (peval t);
+    | term_inr t                 := peval_inr (peval t);
+    (* TODO: Finish the cases below. *)
+    | @term_projtup _ _ t n _ p  := @term_projtup _ _ (peval t) n _ p;
+    | @term_union _ U K t        := @term_union _ U K (peval t);
+    | @term_record _ R ts        := @term_record _ R ts.
 
-  Lemma peval_not_sound {Σ} (t : Term Σ ty_bool) :
-    forall (ι : Valuation Σ),
-      inst (peval_not t) ι = inst (term_not t) ι.
-  Proof. dependent elimination t; cbn; auto. Qed.
+    Lemma peval_neg_sound (t : Term Σ ty_int) :
+      forall (ι : Valuation Σ),
+        inst (peval_neg t) ι = inst (term_neg t) ι.
+    Proof. dependent elimination t; cbn; auto. Qed.
 
-  Lemma peval_inl_sound {Σ σ1 σ2} (t : Term Σ σ1) :
-    forall (ι : Valuation Σ),
-      inst (peval_inl (σ2 := σ2) t) ι = inst (term_inl t) ι.
-  Proof. destruct t; cbn; auto. Qed.
+    Lemma peval_not_sound (t : Term Σ ty_bool) :
+      forall (ι : Valuation Σ),
+        inst (peval_not t) ι = inst (term_not t) ι.
+    Proof. dependent elimination t; cbn; auto. Qed.
 
-  Lemma peval_inr_sound {Σ σ1 σ2} (t : Term Σ σ2) :
-    forall (ι : Valuation Σ),
-      inst (peval_inr (σ1 := σ1) t) ι = inst (term_inr t) ι.
-  Proof. destruct t; cbn; auto. Qed.
+    Lemma peval_inl_sound {σ1 σ2} (t : Term Σ σ1) :
+      forall (ι : Valuation Σ),
+        inst (peval_inl (σ2 := σ2) t) ι = inst (term_inl t) ι.
+    Proof. destruct t; cbn; auto. Qed.
 
-  Lemma peval_sound {Σ σ} (t : Term Σ σ) :
-    forall (ι : Valuation Σ),
-      inst (peval t) ι = inst t ι.
-  Proof.
-    intros ι. symmetry.
-    induction t; cbn;
-      change (inst_term ?t ?ι) with (inst t ι).
-    - reflexivity.
-    - reflexivity.
-    - now rewrite peval_binop_sound, IHt1, IHt2.
-    - now rewrite peval_neg_sound, IHt.
-    - now rewrite peval_not_sound, IHt.
-    - change (Val σ1 + Val σ2)%type with (Val (ty_sum σ1 σ2)).
-      now rewrite peval_inl_sound, IHt.
-    - change (Val σ1 + Val σ2)%type with (Val (ty_sum σ1 σ2)).
-      now rewrite peval_inr_sound, IHt.
-    - now rewrite IHt.
-    - now rewrite IHt.
-    - reflexivity.
-  Qed.
+    Lemma peval_inr_sound {σ1 σ2} (t : Term Σ σ2) :
+      forall (ι : Valuation Σ),
+        inst (peval_inr (σ1 := σ1) t) ι = inst (term_inr t) ι.
+    Proof. destruct t; cbn; auto. Qed.
 
+    Lemma peval_sound [σ] (t : Term Σ σ) :
+      forall (ι : Valuation Σ),
+        inst (peval t) ι = inst t ι.
+    Proof.
+      intros ι. symmetry.
+      induction t; cbn;
+        change (inst_term ?t ?ι) with (inst t ι).
+      - reflexivity.
+      - reflexivity.
+      - now rewrite peval_binop_sound, IHt1, IHt2.
+      - now rewrite peval_neg_sound, IHt.
+      - now rewrite peval_not_sound, IHt.
+      - change (Val σ1 + Val σ2)%type with (Val (ty_sum σ1 σ2)).
+        now rewrite peval_inl_sound, IHt.
+      - change (Val σ1 + Val σ2)%type with (Val (ty_sum σ1 σ2)).
+        now rewrite peval_inr_sound, IHt.
+      - now rewrite IHt.
+      - now rewrite IHt.
+      - reflexivity.
+    Qed.
+
+  End WithLCtx.
 End PartialEvaluationOn.
